proofs/ContextGraph/README.md
@@ -1,39 +1,45 @@
 # Context graphs
 
-This directory introduces an original notion we call *context graph*.
+This directory presents an original notion we call *context graph*.
 
 Informally speaking, a context graph is a graph in which each node can be
-"exploded" in a sense to reveal further graph structure, the nodes of which can
-themselves be exploded, and so on.
+"unfolded" in a sense to reveal further graph structure, the nodes of which can
+themselves be unfolded, and so on.
 
 In the other direction, a context graph is organized into subgraphs which can
-be "collapsed" into single nodes, resulting in a coarser view of the graph which
-can be further collapsed, until ultimately the entire graph has been collapsed
-into a single *root* node.
+be "folded" into single nodes, resulting in a coarser view of the graph which
+can be further folded, until ultimately the entire graph has been folded into
+a single *root* node.
+
+Context graphs permit sharing of substructure, but any such sharing must be
+made explicit: if two nodes share any substructure, there must be an edge
+between them.
 
 Each edge of a context graph is associated with a particular node called its
-*context*. The context of an edge is the node that explodes to reveal that
+*context*. The context of an edge is the node that unfolded to reveal that
 edge. All the edges sharing a context can be considered to belong to the same
-collapsible subgraph.
+foldable subgraph.
 
 Context graphs support two notions of reachability from one node to another:
 
 - `B` is *horizontally reachable* from `A` in context `C` when there is a
-  (possibly empty) path from `A` to `B` consisting only of edges in context `C`.
+  (possibly empty) path from `A` to `B` consisting only of edges in context
+  `C`.
 - `B` is *vertically reachable* from `A` when `A` and `B` are the same node or
   there is a node `C` which is horizontally reachable from `A` in context `A`
   and `B` is vertically reachable from `C`.
 
-Informally speaking, vertical reachability is allowed to explode nodes to reach
-the target (or, equivalently, collapse subgraphs to reach the source), whereas
+Informally speaking, vertical reachability is allowed to unfold nodes to reach
+the target (or, equivalently, fold subgraphs to reach the source), whereas
 horizontal reachability is not.
 
 Every node is required to be vertically reachable from the root.
 
-Context graphs are directed by default, but can be made undirected by
-introducing a symmetry axiom. Context graphs support sharing of substructure in
-the sense that the collapsible subgraphs may contain overlapping nodes (which
-can be exploded into shared subgraphs), although an additional axiom can be
-postulated to forbid that. Context graphs by default do not allow for cyclic
-exploding in which distinct nodes are mutually contained within each other,
-although such models can be admitted by removing the antisymmetry axiom.
+## Variations
+
+- Context graphs are directed by default, but can be made undirected by
+  postulating a symmetry axiom.
+- Context graphs by default do not allow for cyclic unfolding in which multiple
+  nodes are mutually contained within each other, although such models can be
+  admitted by removing the antisymmetry axiom.
+- Sharing of substructure can be forbidden with an additional axiom.
